Rename and new Cannon01proof

proofmode/IProofMode.v
@@ -83,36 +83,32 @@ Section SIM.
     }
   Qed.
 
-  Definition back
-             (r g: forall R_src R_tgt
-                          (Q: Any.t -> Any.t -> R_src -> R_tgt -> iProp)
-                          (ctx: Σ),
-                 option Ord.t -> bool -> bool -> Any.t * itree hEs R_src -> Any.t * itree Es R_tgt -> Prop)
+  Definition isim
+             '(r, g, f_src, f_tgt)
              {R_src R_tgt}
              (Q: Any.t -> Any.t -> R_src -> R_tgt -> iProp)
              (fuel: option Ord.t)
-             (f_src f_tgt: bool)
              (st_src: Any.t * itree hEs R_src)
              (st_tgt: Any.t * itree Es R_tgt): iProp :=
     fun res =>
       forall ctx (WF: URA.wf (res ⋅ ctx)),
         gpaco9 (_hsim) (cpn9 _hsim) r g _ _ Q ctx fuel f_src f_tgt st_src st_tgt.
 
-  Lemma back_init
+  Lemma isim_init
         R_src R_tgt (Q: Any.t -> Any.t -> R_src -> R_tgt -> iProp)
         P r g ctx fuel f_src f_tgt st_src st_tgt itr_src itr_tgt
         (ENTAIL: bi_entails
                    P
-                   (back r g Q fuel f_src f_tgt (st_src, itr_src) (st_tgt, itr_tgt)))
+                   (isim (r, g, f_src, f_tgt) Q fuel (st_src, itr_src) (st_tgt, itr_tgt)))
         (CUR: current_iProp ctx P)
     :
       gpaco9 _hsim (cpn9 _hsim) r g _ _ Q ctx fuel f_src f_tgt (st_src, itr_src) (st_tgt, itr_tgt).
   Proof.
     eapply current_iProp_entail in ENTAIL; eauto.
-    inv ENTAIL. unfold back in IPROP. eapply IPROP; eauto.
+    inv ENTAIL. unfold isim in IPROP. eapply IPROP; eauto.
   Qed.
 
-  Lemma back_final
+  Lemma isim_final
         R_src R_tgt (Q: Any.t -> Any.t -> R_src -> R_tgt -> iProp)
         P r g fuel f_src f_tgt st_src st_tgt itr_src itr_tgt
         (SIM: forall ctx
@@ -121,47 +117,47 @@ Section SIM.
     :
       bi_entails
         P
-        (back r g Q fuel f_src f_tgt (st_src, itr_src) (st_tgt, itr_tgt)).
+        (isim (r, g, f_src, f_tgt) Q fuel (st_src, itr_src) (st_tgt, itr_tgt)).
   Proof.
     uipropall. ii. eapply SIM. econs; eauto.
   Qed.
 
-  Lemma back_current
+  Lemma isim_current
         R_src R_tgt (Q: Any.t -> Any.t -> R_src -> R_tgt -> iProp)
         r g fuel ctx f_src f_tgt st_src st_tgt itr_src itr_tgt
-        (CUR: current_iProp ctx (back r g Q fuel f_src f_tgt (st_src, itr_src) (st_tgt, itr_tgt)))
+        (CUR: current_iProp ctx (isim (r, g, f_src, f_tgt) Q fuel (st_src, itr_src) (st_tgt, itr_tgt)))
     :
       gpaco9 _hsim (cpn9 _hsim) r g _ _ Q ctx fuel f_src f_tgt (st_src, itr_src) (st_tgt, itr_tgt).
   Proof.
     inv CUR. eapply IPROP; eauto.
   Qed.
 
-  Lemma back_mono R_src R_tgt
+  Lemma isim_mono R_src R_tgt
         (Q0 Q1: Any.t -> Any.t -> R_src -> R_tgt -> iProp)
         r g fuel f_src f_tgt st_src itr_src st_tgt itr_tgt
         (MONO: forall st_src st_tgt ret_src ret_tgt,
             (bi_entails (Q0 st_src st_tgt ret_src ret_tgt) (#=> Q1 st_src st_tgt ret_src ret_tgt)))
     :
       bi_entails
-        (back r g Q0 fuel f_src f_tgt (st_src, itr_src) (st_tgt, itr_tgt))
-        (back r g Q1 fuel f_src f_tgt (st_src, itr_src) (st_tgt, itr_tgt)).
+        (isim (r, g, f_src, f_tgt) Q0 fuel (st_src, itr_src) (st_tgt, itr_tgt))
+        (isim (r, g, f_src, f_tgt) Q1 fuel (st_src, itr_src) (st_tgt, itr_tgt)).
   Proof.
     red. unfold Entails. autorewrite with iprop.
-    unfold back in *. i. hexploit H; eauto. i.
+    unfold isim in *. i. hexploit H; eauto. i.
     guclo hmonoC_spec. econs; eauto.
   Qed.
 
-  Lemma back_wand R_src R_tgt
+  Lemma isim_wand R_src R_tgt
         (Q0 Q1: Any.t -> Any.t -> R_src -> R_tgt -> iProp)
         r g fuel f_src f_tgt st_src itr_src st_tgt itr_tgt
     :
       bi_entails
         ((∀ st_src st_tgt ret_src ret_tgt,
-             ((Q0 st_src st_tgt ret_src ret_tgt) -∗ (#=> Q1 st_src st_tgt ret_src ret_tgt))) ** (back r g Q0 fuel f_src f_tgt (st_src, itr_src) (st_tgt, itr_tgt)))
-        (back r g Q1 fuel f_src f_tgt (st_src, itr_src) (st_tgt, itr_tgt)).
+             ((Q0 st_src st_tgt ret_src ret_tgt) -∗ (#=> Q1 st_src st_tgt ret_src ret_tgt))) ** (isim (r, g, f_src, f_tgt) Q0 fuel (st_src, itr_src) (st_tgt, itr_tgt)))
+        (isim (r, g, f_src, f_tgt) Q1 fuel (st_src, itr_src) (st_tgt, itr_tgt)).
   Proof.
     red. unfold Entails. autorewrite with iprop.
-    unfold back in *. i.
+    unfold isim in *. i.
     red in H. unfold Sepconj in H. autorewrite with iprop in H.
     des. clarify. eapply from_semantic in H0. hexploit (H1 (ctx ⋅ a)).
     { r_wf WF0. }
@@ -174,150 +170,100 @@ Section SIM.
     iMod "H1". iApply "H1". iApply "H0".
   Qed.
 
-  Lemma back_upd R_src R_tgt
+  Lemma isim_upd R_src R_tgt
         (Q: Any.t -> Any.t -> R_src -> R_tgt -> iProp)
         r g fuel f_src f_tgt st_src st_tgt
     :
       bi_entails
-        (#=> (back r g Q fuel f_src f_tgt st_src st_tgt))
-        (back r g Q fuel f_src f_tgt st_src st_tgt).
+        (#=> (isim (r, g, f_src, f_tgt) Q fuel st_src st_tgt))
+        (isim (r, g, f_src, f_tgt) Q fuel st_src st_tgt).
   Proof.
     red. unfold Entails. autorewrite with iprop.
-    unfold back in *. i.
+    unfold isim in *. i.
     red in H. unfold bi_bupd_bupd in H. ss. unfold Upd in H. autorewrite with iprop in H.
     hexploit H; eauto. i. des.
     hexploit H1; eauto.
   Qed.
 
-  Lemma back_bind R_src R_tgt S_src S_tgt
+  Lemma isim_bind R_src R_tgt S_src S_tgt
         (Q: Any.t -> Any.t -> R_src -> R_tgt -> iProp)
         r g fuel f_src f_tgt st_src (itr_src: itree hEs S_src)
         ktr_src st_tgt (itr_tgt: itree Es S_tgt) ktr_tgt
     :
       bi_entails
-        (back r g (fun st_src st_tgt ret_src ret_tgt => back r g Q None false false (st_src, ktr_src ret_src) (st_tgt, ktr_tgt ret_tgt)) fuel f_src f_tgt (st_src, itr_src) (st_tgt, itr_tgt))
-        (back r g Q fuel f_src f_tgt (st_src, itr_src >>= ktr_src) (st_tgt, itr_tgt >>= ktr_tgt)).
+        (isim (r, g, f_src, f_tgt) (fun st_src st_tgt ret_src ret_tgt => isim (r, g, false, false) Q None (st_src, ktr_src ret_src) (st_tgt, ktr_tgt ret_tgt)) fuel (st_src, itr_src) (st_tgt, itr_tgt))
+        (isim (r, g, f_src, f_tgt) Q fuel (st_src, itr_src >>= ktr_src) (st_tgt, itr_tgt >>= ktr_tgt)).
   Proof.
     red. unfold Entails. autorewrite with iprop.
-    unfold back in *. i.
+    unfold isim in *. i.
     guclo hbindC_spec. econs.
     { eapply H; eauto. }
     i. inv POST. eapply IPROP. eauto.
   Qed.
 
-  Lemma back_bind_left R_src R_tgt S_src
+  Lemma isim_bind_left R_src R_tgt S_src
         (Q: Any.t -> Any.t -> R_src -> R_tgt -> iProp)
         r g fuel f_src f_tgt st_src (itr_src: itree hEs S_src)
         ktr_src st_tgt itr_tgt
     :
       bi_entails
-        (back r g (fun st_src st_tgt ret_src ret_tgt => back r g Q None false false (st_src, ktr_src ret_src) (st_tgt, itr_tgt)) fuel f_src f_tgt (st_src, itr_src) (st_tgt, Ret tt))
-        (back r g Q fuel f_src f_tgt (st_src, itr_src >>= ktr_src) (st_tgt, itr_tgt)).
+        (isim (r, g, f_src, f_tgt) (fun st_src st_tgt ret_src ret_tgt => isim (r, g, false, false) Q None (st_src, ktr_src ret_src) (st_tgt, itr_tgt)) fuel (st_src, itr_src) (st_tgt, Ret tt))
+        (isim (r, g, f_src, f_tgt) Q fuel (st_src, itr_src >>= ktr_src) (st_tgt, itr_tgt)).
   Proof.
     iIntros "H".
     assert (EQ: itr_tgt = Ret tt >>= fun _ => itr_tgt).
     { grind. }
-    rewrite EQ. iApply back_bind. rewrite <- EQ. iApply "H".
+    rewrite EQ. iApply isim_bind. rewrite <- EQ. iApply "H".
   Qed.
 
-  Lemma back_bind_right R_src R_tgt S_tgt
+  Lemma isim_bind_right R_src R_tgt S_tgt
         (Q: Any.t -> Any.t -> R_src -> R_tgt -> iProp)
         r g fuel f_src f_tgt st_src itr_src
         st_tgt (itr_tgt: itree Es S_tgt) ktr_tgt
     :
       bi_entails
-        (back r g (fun st_src st_tgt ret_src ret_tgt => back r g Q None false false (st_src, itr_src) (st_tgt, ktr_tgt ret_tgt)) fuel f_src f_tgt (st_src, Ret tt) (st_tgt, itr_tgt))
-        (back r g Q fuel f_src f_tgt (st_src, itr_src) (st_tgt, itr_tgt >>= ktr_tgt)).
+        (isim (r, g, f_src, f_tgt) (fun st_src st_tgt ret_src ret_tgt => isim (r, g, false, false) Q None (st_src, itr_src) (st_tgt, ktr_tgt ret_tgt)) fuel (st_src, Ret tt) (st_tgt, itr_tgt))
+        (isim (r, g, f_src, f_tgt) Q fuel (st_src, itr_src) (st_tgt, itr_tgt >>= ktr_tgt)).
   Proof.
     iIntros "H".
     assert (EQ: itr_src = Ret tt >>= fun _ => itr_src).
     { grind. }
-    rewrite EQ. iApply back_bind. rewrite <- EQ. iApply "H".
+    rewrite EQ. iApply isim_bind. rewrite <- EQ. iApply "H".
   Qed.
 
-  Lemma back_bind_right_pure R_src R_tgt S_tgt
+  Lemma isim_bind_right_pure R_src R_tgt S_tgt
         (Q: Any.t -> Any.t -> R_src -> R_tgt -> iProp)
         r g fuel f_src f_tgt st_src itr_src
         st_tgt (itr_tgt: itree Es S_tgt) ktr_tgt
     :
       bi_entails
-        (back r g (fun st_src st_tgt ret_src ret_tgt => back r g Q fuel false false (st_src, itr_src) (st_tgt, ktr_tgt ret_tgt)) None f_src f_tgt (st_src, Ret tt) (st_tgt, itr_tgt))
-        (back r g Q fuel f_src f_tgt (st_src, itr_src) (st_tgt, itr_tgt >>= ktr_tgt)).
+        (isim (r, g, f_src, f_tgt) (fun st_src st_tgt ret_src ret_tgt => isim (r, g, false, false) Q fuel (st_src, itr_src) (st_tgt, ktr_tgt ret_tgt)) None (st_src, Ret tt) (st_tgt, itr_tgt))
+        (isim (r, g, f_src, f_tgt) Q fuel (st_src, itr_src) (st_tgt, itr_tgt >>= ktr_tgt)).
   Proof.
     red. unfold Entails. autorewrite with iprop.
-    unfold back in *. i.
+    unfold isim in *. i.
     guclo hbind_rightC_spec. econs.
     { eapply H; eauto. }
     i. inv POST. eapply IPROP. eauto.
   Qed.
 
-  Lemma back_progress R_src R_tgt
-        (Q: Any.t -> Any.t -> R_src -> R_tgt -> iProp)
-        r g fuel st_src itr_src st_tgt itr_tgt
-    :
-      bi_entails
-        (back g g Q fuel false false (st_src, itr_src) (st_tgt, itr_tgt))
-        (back r g Q fuel true true (st_src, itr_src) (st_tgt, itr_tgt)).
-  Proof.
-    eapply back_final. i. eapply back_current in CUR.
-    eapply hsim_progress_flag. auto.
-  Qed.
-
-  Lemma back_flag_mon
-        fuel0 f_src0 f_tgt0
-        R_src R_tgt
-        (Q: Any.t -> Any.t -> R_src -> R_tgt -> iProp)
-        r g st_src itr_src st_tgt itr_tgt
-        fuel1 f_src1 f_tgt1
-        (SRC: f_src0 = true -> f_src1 = true)
-        (TGT: f_tgt0 = true -> f_tgt1 = true)
-        (FUEL: option_Ord_le fuel0 fuel1)
-    :
-      bi_entails
-        (back r g Q fuel0 f_src0 f_tgt0 (st_src, itr_src) (st_tgt, itr_tgt))
-        (back r g Q fuel1 f_src1 f_tgt1 (st_src, itr_src) (st_tgt, itr_tgt)).
-  Proof.
-    eapply back_final. i. eapply back_current in CUR.
-    guclo hflagC_spec. econs; eauto.
-  Qed.
-
-  Lemma back_split_aux R_src R_tgt S_tgt
+  Lemma isim_split_aux R_src R_tgt S_tgt
         (Q: Any.t -> Any.t -> R_src -> R_tgt -> iProp)
         r g st_src itr_src st_tgt (itr_tgt: itree Es S_tgt) ktr_tgt
         fuel0 fuel1 f_src f_tgt
     :
       bi_entails
-        (back r g (fun st_src st_tgt _ ret_tgt => back r g Q (Some fuel1) false false (st_src, itr_src) (st_tgt, ktr_tgt ret_tgt)) (Some fuel0) f_src f_tgt (st_src, Ret tt) (st_tgt, itr_tgt))
-        (back r g Q (Some (fuel1 + fuel0)%ord) f_src f_tgt (st_src, itr_src) (st_tgt, itr_tgt >>= ktr_tgt)).
+        (isim (r, g, f_src, f_tgt) (fun st_src st_tgt _ ret_tgt => isim (r, g, false, false) Q (Some fuel1) (st_src, itr_src) (st_tgt, ktr_tgt ret_tgt)) (Some fuel0) (st_src, Ret tt) (st_tgt, itr_tgt))
+        (isim (r, g, f_src, f_tgt) Q (Some (fuel1 + fuel0)%ord) (st_src, itr_src) (st_tgt, itr_tgt >>= ktr_tgt)).
   Proof.
     red. unfold Entails. autorewrite with iprop.
-    unfold back in *. i.
+    unfold isim in *. i.
     guclo hsplitC_spec. econs.
     { eapply H; eauto. }
     i. inv POST. eapply IPROP. eauto.
   Qed.
 
-  Lemma back_split
-        fuel0 fuel1
-        R_src R_tgt S_tgt
-        (Q: Any.t -> Any.t -> R_src -> R_tgt -> iProp)
-        r g st_src itr_src st_tgt (itr_tgt: itree Es S_tgt) ktr_tgt
-        fuel f_src f_tgt
-        (FUEL: (fuel1 + fuel0 <= fuel)%ord)
-    :
-      bi_entails
-        (back r g (fun st_src st_tgt _ ret_tgt => back r g Q (Some fuel1) false false (st_src, itr_src) (st_tgt, ktr_tgt ret_tgt)) (Some fuel0) f_src f_tgt (st_src, Ret tt) (st_tgt, itr_tgt))
-        (back r g Q (Some fuel) f_src f_tgt (st_src, itr_src) (st_tgt, itr_tgt >>= ktr_tgt)).
-  Proof.
-    iIntros "H".
-    iApply back_flag_mon.
-    { eauto. }
-    { eauto. }
-    { instantiate (1:=Some (fuel1 + fuel0)%ord). ss. }
-    iApply back_split_aux. auto.
-  Qed.
-
-  Lemma back_call_impure
+  Lemma isim_call_impure
         pre post w0
         R_src R_tgt
         (Q: Any.t -> Any.t -> R_src -> R_tgt -> iProp)
@@ -328,11 +274,11 @@ Section SIM.
         ((inv_with le I w0 st_src st_tgt)
            ** (pre: iProp)
            ** (∀ st_src st_tgt ret_src ret_tgt,
-                  inv_with le I w0 st_src st_tgt -* (post ret_src ret_tgt: iProp) -* back g g Q None true true (st_src, ktr_src ret_src) (st_tgt, ktr_tgt ret_tgt)))
-        (back r g Q fuel f_src f_tgt (st_src, trigger (Call fn arg_src) >>= ktr_src) (st_tgt, trigger (Call fn arg_tgt) >>= ktr_tgt)).
+                  inv_with le I w0 st_src st_tgt -* (post ret_src ret_tgt: iProp) -* isim (g, g, true, true) Q None (st_src, ktr_src ret_src) (st_tgt, ktr_tgt ret_tgt)))
+        (isim (r, g, f_src, f_tgt) Q fuel (st_src, trigger (Call fn arg_src) >>= ktr_src) (st_tgt, trigger (Call fn arg_tgt) >>= ktr_tgt)).
   Proof.
     red. unfold Entails. autorewrite with iprop.
-    unfold back at 2. i.
+    unfold isim at 2. i.
     match (type of H) with
     | ?P _ =>
       assert (CUR: current_iProp ctx P)
@@ -358,14 +304,14 @@ Section SIM.
     mAssert _ with "A".
     { iApply (POST with "A"). }
     mUpd "A2".
-    mAssert (back g g Q None true true (st_src1, ktr_src ret_src)
+    mAssert (isim (g, g, true, true) Q None (st_src1, ktr_src ret_src)
                   (st_tgt1, ktr_tgt ret_tgt)) with "*".
     { iApply ("H" with "A1 A2"). }
     inv ACC. red in IPROP. uipropall. des. subst.
     eapply IPROP0. eapply URA.wf_mon. instantiate (1:=b). r_wf GWF.
   Qed.
 
-  Lemma back_call_pure
+  Lemma isim_call_pure
         pre post w0 fuel1
         R_src R_tgt
         (Q: Any.t -> Any.t -> R_src -> R_tgt -> iProp)
@@ -379,11 +325,11 @@ Section SIM.
                   ** (pre: iProp)
                   **
                   (∀ st_src st_tgt ret_src ret_tgt,
-                      ((inv_with le I w0 st_src st_tgt) ** (post ret_src ret_tgt: iProp)) -* back g g Q (Some fuel1) true true (st_src, itr_src) (st_tgt, ktr_tgt ret_tgt)))
-        (back r g Q (Some fuel0) f_src f_tgt (st_src, itr_src) (st_tgt, trigger (Call fn arg_tgt) >>= ktr_tgt)).
+                      ((inv_with le I w0 st_src st_tgt) ** (post ret_src ret_tgt: iProp)) -* isim (g, g, true, true) Q (Some fuel1) (st_src, itr_src) (st_tgt, ktr_tgt ret_tgt)))
+        (isim (r, g, f_src, f_tgt) Q (Some fuel0) (st_src, itr_src) (st_tgt, trigger (Call fn arg_tgt) >>= ktr_tgt)).
   Proof.
     red. unfold Entails. autorewrite with iprop.
-    unfold back at 2. i.
+    unfold isim at 2. i.
     match (type of H) with
     | ?P _ =>
       assert (CUR: current_iProp ctx P)
@@ -409,13 +355,78 @@ Section SIM.
     mAssert _ with "A".
     { iApply (POST with "A"). }
     mUpd "A2".
-    mAssert (back g g Q (Some fuel1) true true (st_src1, itr_src) (st_tgt1, ktr_tgt ret_tgt)) with "*".
+    mAssert (isim (g, g, true, true) Q (Some fuel1) (st_src1, itr_src) (st_tgt1, ktr_tgt ret_tgt)) with "*".
     { iApply "H". iSplitR "A2"; auto. }
     inv ACC. red in IPROP. uipropall. des. subst. eapply IPROP0.
     eapply URA.wf_mon. instantiate (1:=b). r_wf GWF.
   Qed.
 
-  Lemma back_ret
+  Lemma isim_apc
+        R_src R_tgt
+        (Q: Any.t -> Any.t -> R_src -> R_tgt -> iProp)
+        r g f_src f_tgt st_src st_tgt ktr_src itr_tgt
+        fuel0
+    :
+      bi_entails
+        (∃ fuel1, isim (r, g, true, f_tgt) Q fuel1 (st_src, ktr_src tt) (st_tgt, itr_tgt))
+        (isim (r, g, f_src, f_tgt) Q fuel0 (st_src, trigger hAPC >>= ktr_src) (st_tgt, itr_tgt)).
+  Proof.
+    eapply isim_final. i.
+    inv CUR. red in IPROP. uipropall. des.
+    eapply hsimC_uclo. econs; eauto.
+  Qed.
+
+  Lemma isim_progress R_src R_tgt
+        (Q: Any.t -> Any.t -> R_src -> R_tgt -> iProp)
+        r g fuel st_src itr_src st_tgt itr_tgt
+    :
+      bi_entails
+        (isim (g, g, false, false) Q fuel (st_src, itr_src) (st_tgt, itr_tgt))
+        (isim (r, g, true, true) Q fuel (st_src, itr_src) (st_tgt, itr_tgt)).
+  Proof.
+    eapply isim_final. i. eapply isim_current in CUR.
+    eapply hsim_progress_flag. auto.
+  Qed.
+
+  Lemma isim_flag_mon
+        fuel0 f_src0 f_tgt0
+        R_src R_tgt
+        (Q: Any.t -> Any.t -> R_src -> R_tgt -> iProp)
+        r g st_src itr_src st_tgt itr_tgt
+        fuel1 f_src1 f_tgt1
+        (SRC: f_src0 = true -> f_src1 = true)
+        (TGT: f_tgt0 = true -> f_tgt1 = true)
+        (FUEL: option_Ord_le fuel0 fuel1)
+    :
+      bi_entails
+        (isim (r, g, f_src0, f_tgt0) Q fuel0 (st_src, itr_src) (st_tgt, itr_tgt))
+        (isim (r, g, f_src1, f_tgt1) Q fuel1 (st_src, itr_src) (st_tgt, itr_tgt)).
+  Proof.
+    eapply isim_final. i. eapply isim_current in CUR.
+    guclo hflagC_spec. econs; eauto.
+  Qed.
+
+  Lemma isim_split
+        fuel0 fuel1
+        R_src R_tgt S_tgt
+        (Q: Any.t -> Any.t -> R_src -> R_tgt -> iProp)
+        r g st_src itr_src st_tgt (itr_tgt: itree Es S_tgt) ktr_tgt
+        fuel f_src f_tgt
+        (FUEL: (fuel1 + fuel0 <= fuel)%ord)
+    :
+      bi_entails
+        (isim (r, g, f_src, f_tgt) (fun st_src st_tgt _ ret_tgt => isim (r, g, false, false) Q (Some fuel1) (st_src, itr_src) (st_tgt, ktr_tgt ret_tgt)) (Some fuel0) (st_src, Ret tt) (st_tgt, itr_tgt))
+        (isim (r, g, f_src, f_tgt) Q (Some fuel) (st_src, itr_src) (st_tgt, itr_tgt >>= ktr_tgt)).
+  Proof.
+    iIntros "H".
+    iApply isim_flag_mon.
+    { eauto. }
+    { eauto. }
+    { instantiate (1:=Some (fuel1 + fuel0)%ord). ss. }
+    iApply isim_split_aux. auto.
+  Qed.
+
+  Lemma isim_ret
         R_src R_tgt (Q: Any.t -> Any.t -> R_src -> R_tgt -> iProp)
         r g
         v_src v_tgt
@@ -424,42 +435,27 @@ Section SIM.
     :
       bi_entails
         (Q st_src st_tgt v_src v_tgt)
-        (back r g Q fuel f_src f_tgt (st_src, Ret v_src) (st_tgt, (Ret v_tgt))).
+        (isim (r, g, f_src, f_tgt) Q fuel (st_src, Ret v_src) (st_tgt, (Ret v_tgt))).
   Proof.
-    eapply back_final. i.
+    eapply isim_final. i.
     eapply hsimC_uclo. econs; eauto.
   Qed.
 
-  Lemma back_apc
-        R_src R_tgt
-        (Q: Any.t -> Any.t -> R_src -> R_tgt -> iProp)
-        r g f_src f_tgt st_src st_tgt ktr_src itr_tgt
-        fuel0
-    :
-      bi_entails
-        (∃ fuel1, back r g Q fuel1 true f_tgt (st_src, ktr_src tt) (st_tgt, itr_tgt))
-        (back r g Q fuel0 f_src f_tgt (st_src, trigger hAPC >>= ktr_src) (st_tgt, itr_tgt)).
-  Proof.
-    eapply back_final. i.
-    inv CUR. red in IPROP. uipropall. des.
-    eapply hsimC_uclo. econs; eauto.
-  Qed.
-
-  Lemma back_apc_trigger
+  Lemma isim_apc_trigger
         R_tgt
         (Q: Any.t -> Any.t -> unit -> R_tgt -> iProp)
         r g f_src f_tgt st_src st_tgt itr_tgt
         fuel0
     :
       bi_entails
-        (∃ fuel1, back r g Q fuel1 true f_tgt (st_src, Ret tt) (st_tgt, itr_tgt))
-        (back r g Q fuel0 f_src f_tgt (st_src, trigger hAPC) (st_tgt, itr_tgt)).
+        (∃ fuel1, isim (r, g, true, f_tgt) Q fuel1 (st_src, Ret tt) (st_tgt, itr_tgt))
+        (isim (r, g, f_src, f_tgt) Q fuel0 (st_src, trigger hAPC) (st_tgt, itr_tgt)).
   Proof.
     erewrite (@idK_spec _ _ (trigger (hAPC))).
-    iIntros "H". iApply back_apc. iExact "H".
+    iIntros "H". iApply isim_apc. iExact "H".
   Qed.
 
-  Lemma back_call_impure_trigger
+  Lemma isim_call_impure_trigger
         pre post w0
         (Q: Any.t -> Any.t -> Any.t -> Any.t -> iProp)
         r g fuel f_src f_tgt st_src st_tgt fn arg_src arg_tgt
@@ -471,17 +467,17 @@ Section SIM.
            **
            (∀ st_src st_tgt ret_src ret_tgt,
                (inv_with le I w0 st_src st_tgt) -* (post ret_src ret_tgt: iProp) -* Q st_src st_tgt ret_src ret_tgt))
-        (back r g Q fuel f_src f_tgt (st_src, trigger (Call fn arg_src)) (st_tgt, trigger (Call fn arg_tgt))).
+        (isim (r, g, f_src, f_tgt) Q fuel (st_src, trigger (Call fn arg_src)) (st_tgt, trigger (Call fn arg_tgt))).
   Proof.
     erewrite (@idK_spec _ _ (trigger (Call fn arg_src))).
     erewrite (@idK_spec _ _ (trigger (Call fn arg_tgt))).
-    iIntros "H". iApply back_call_impure; eauto.
+    iIntros "H". iApply isim_call_impure; eauto.
     iDestruct "H" as "[H0 H1]". iSplitL "H0"; auto.
     iIntros (st_src0 st_tgt0 ret_src ret_tgt) "H0 H2".
-    iApply back_ret. iApply ("H1" with "H0 H2").
+    iApply isim_ret. iApply ("H1" with "H0 H2").
   Qed.
 
-  Lemma back_call_pure_trigger
+  Lemma isim_call_pure_trigger
         pre post w0
         (Q: Any.t -> Any.t -> unit -> Any.t -> iProp)
         r g f_src f_tgt st_src st_tgt fn arg_src arg_tgt
@@ -493,343 +489,343 @@ Section SIM.
            **
            (∀ st_src st_tgt ret_src ret_tgt,
                (inv_with le I w0 st_src st_tgt) -* (post ret_src ret_tgt: iProp) -* Q st_src st_tgt tt ret_tgt))
-        (back r g Q (Some (1: Ord.t)) f_src f_tgt (st_src, Ret tt) (st_tgt, trigger (Call fn arg_tgt))).
+        (isim (r, g, f_src, f_tgt) Q (Some (1: Ord.t)) (st_src, Ret tt) (st_tgt, trigger (Call fn arg_tgt))).
   Proof.
     erewrite (@idK_spec _ _ (trigger (Call fn arg_tgt))).
-    iIntros "H". iApply back_call_pure; eauto.
+    iIntros "H". iApply isim_call_pure; eauto.
     { oauto. }
     iDestruct "H" as "[H0 H1]". iSplitL "H0"; auto.
     iIntros (st_src0 st_tgt0 ret_src ret_tgt) "[H0 H2]".
-    iApply back_ret. iApply ("H1" with "H0 H2").
+    iApply isim_ret. iApply ("H1" with "H0 H2").
   Qed.
 
-  Global Instance iProp_back_absorbing
+  Global Instance iProp_isim_absorbing
          R_src R_tgt r g (Q: Any.t -> Any.t -> R_src -> R_tgt -> iProp)
          fuel f_src f_tgt st_src st_tgt:
-    Absorbing (back r g Q fuel f_src f_tgt st_src st_tgt).
+    Absorbing (isim (r, g, f_src, f_tgt) Q fuel st_src st_tgt).
   Proof.
     unfold Absorbing. unfold bi_absorbingly.
-    iIntros "[H0 H1]". iApply back_upd.
+    iIntros "[H0 H1]". iApply isim_upd.
     iDestruct "H0" as "%". iModIntro. iApply "H1".
   Qed.
 
-  Global Instance iProp_back_elim_upd
+  Global Instance iProp_isim_elim_upd
          R_src R_tgt r g (Q: Any.t -> Any.t -> R_src -> R_tgt -> iProp)
          fuel f_src f_tgt st_src st_tgt
          P:
-    ElimModal True false false (#=> P) P (back r g Q fuel f_src f_tgt st_src st_tgt) (back r g Q fuel f_src f_tgt st_src st_tgt).
+    ElimModal True false false (#=> P) P (isim (r, g, f_src, f_tgt) Q fuel st_src st_tgt) (isim (r, g, f_src, f_tgt) Q fuel st_src st_tgt).
   Proof.
     unfold ElimModal. i. iIntros "[H0 H1]".
-    iApply back_upd. iMod "H0". iModIntro.
+    iApply isim_upd. iMod "H0". iModIntro.
     iApply "H1". iApply "H0".
   Qed.
 
-  Lemma back_syscall
+  Lemma isim_syscall
         R_src R_tgt
         (Q: Any.t -> Any.t -> R_src -> R_tgt -> iProp)
         fn arg rvs
         r g fuel f_src f_tgt st_src st_tgt ktr_src ktr_tgt
     :
       bi_entails
-        (∀ ret, back g g Q None true true (st_src, ktr_src ret) (st_tgt, ktr_tgt ret))
-        (back r g Q fuel f_src f_tgt (st_src, trigger (Syscall fn arg rvs) >>= ktr_src) (st_tgt, trigger (Syscall fn arg rvs) >>= ktr_tgt)).
+        (∀ ret, isim (g, g, true, true) Q None (st_src, ktr_src ret) (st_tgt, ktr_tgt ret))
+        (isim (r, g, f_src, f_tgt) Q fuel (st_src, trigger (Syscall fn arg rvs) >>= ktr_src) (st_tgt, trigger (Syscall fn arg rvs) >>= ktr_tgt)).
   Proof.
-    eapply back_final. i. eapply hsimC_uclo. econs; eauto.
+    eapply isim_final. i. eapply hsimC_uclo. econs; eauto.
     i. inv CUR. red in IPROP. uipropall. eapply IPROP; eauto.
   Qed.
 
-  Lemma back_syscall_trigger
+  Lemma isim_syscall_trigger
         (Q: Any.t -> Any.t -> Any.t -> Any.t -> iProp)
         fn arg_src arg_tgt rvs
         r g fuel f_src f_tgt st_src st_tgt
     :
       bi_entails
         (⌜arg_src = arg_tgt⌝ ** ∀ ret, Q st_src st_tgt ret ret)
-        (back r g Q fuel f_src f_tgt (st_src, trigger (Syscall fn arg_src rvs)) (st_tgt, trigger (Syscall fn arg_tgt rvs))).
+        (isim (r, g, f_src, f_tgt) Q fuel (st_src, trigger (Syscall fn arg_src rvs)) (st_tgt, trigger (Syscall fn arg_tgt rvs))).
   Proof.
     erewrite (@idK_spec _ _ (trigger (Syscall fn arg_src rvs))).
     erewrite (@idK_spec _ _ (trigger (Syscall fn arg_tgt rvs))).
     iIntros "[% H1]". subst.
-    iApply back_syscall. iIntros (ret).
-    iApply back_ret. iApply "H1".
+    iApply isim_syscall. iIntros (ret).
+    iApply isim_ret. iApply "H1".
   Qed.
 
-  Lemma back_tau_src
+  Lemma isim_tau_src
         R_src R_tgt
         (Q: Any.t -> Any.t -> R_src -> R_tgt -> iProp)
         r g fuel f_src f_tgt st_src st_tgt itr_src itr_tgt
     :
       bi_entails
-        (back r g Q None true f_tgt (st_src, itr_src) (st_tgt, itr_tgt))
-        (back r g Q fuel f_src f_tgt (st_src, tau;; itr_src) (st_tgt, itr_tgt)).
+        (isim (r, g, true, f_tgt) Q None (st_src, itr_src) (st_tgt, itr_tgt))
+        (isim (r, g, f_src, f_tgt) Q fuel (st_src, tau;; itr_src) (st_tgt, itr_tgt)).
   Proof.
-    eapply back_final. i. eapply hsimC_uclo. econs; eauto.
-    eapply back_current; eauto.
+    eapply isim_final. i. eapply hsimC_uclo. econs; eauto.
+    eapply isim_current; eauto.
   Qed.
 
-  Lemma back_tau_tgt
+  Lemma isim_tau_tgt
         R_src R_tgt
         (Q: Any.t -> Any.t -> R_src -> R_tgt -> iProp)
         r g fuel f_src f_tgt st_src st_tgt itr_src itr_tgt
     :
       bi_entails
-        (back r g Q fuel f_src true (st_src, itr_src) (st_tgt, itr_tgt))
-        (back r g Q fuel f_src f_tgt (st_src, itr_src) (st_tgt, tau;; itr_tgt)).
+        (isim (r, g, f_src, true) Q fuel (st_src, itr_src) (st_tgt, itr_tgt))
+        (isim (r, g, f_src, f_tgt) Q fuel (st_src, itr_src) (st_tgt, tau;; itr_tgt)).
   Proof.
-    eapply back_final. i. eapply hsimC_uclo. econs; eauto.
-    eapply back_current; eauto.
+    eapply isim_final. i. eapply hsimC_uclo. econs; eauto.
+    eapply isim_current; eauto.
   Qed.
 
-  Lemma back_choose_src
+  Lemma isim_choose_src
         R_src R_tgt
         (Q: Any.t -> Any.t -> R_src -> R_tgt -> iProp)
         r g fuel f_src f_tgt st_src st_tgt X ktr_src itr_tgt
     :
       bi_entails
-        (∃ x, back r g Q None true f_tgt (st_src, ktr_src x) (st_tgt, itr_tgt))
-        (back r g Q fuel f_src f_tgt (st_src, trigger (Choose X) >>= ktr_src) (st_tgt, itr_tgt)).
+        (∃ x, isim (r, g, true, f_tgt) Q None (st_src, ktr_src x) (st_tgt, itr_tgt))
+        (isim (r, g, f_src, f_tgt) Q fuel (st_src, trigger (Choose X) >>= ktr_src) (st_tgt, itr_tgt)).
   Proof.
-    eapply back_final. i. eapply hsimC_uclo. econs; eauto.
+    eapply isim_final. i. eapply hsimC_uclo. econs; eauto.
     inv CUR. red in IPROP. uipropall. des. esplits. eapply IPROP; eauto.
   Qed.
 
-  Lemma back_choose_src_trigger
+  Lemma isim_choose_src_trigger
         X R_tgt
         (Q: Any.t -> Any.t -> X -> R_tgt -> iProp)
         r g fuel f_src f_tgt st_src st_tgt itr_tgt
     :
       bi_entails
-        (∃ x, back r g Q None true f_tgt (st_src, Ret x) (st_tgt, itr_tgt))
-        (back r g Q fuel f_src f_tgt (st_src, trigger (Choose X)) (st_tgt, itr_tgt)).
+        (∃ x, isim (r, g, true, f_tgt) Q None (st_src, Ret x) (st_tgt, itr_tgt))
+        (isim (r, g, f_src, f_tgt) Q fuel (st_src, trigger (Choose X)) (st_tgt, itr_tgt)).
   Proof.
     erewrite (@idK_spec _ _ (trigger (Choose X))).
-    iIntros "H". iApply back_choose_src.
+    iIntros "H". iApply isim_choose_src.
     iDestruct "H" as (x) "H". iExists x. auto.
   Qed.
 
-  Lemma back_choose_tgt
+  Lemma isim_choose_tgt
         R_src R_tgt
         (Q: Any.t -> Any.t -> R_src -> R_tgt -> iProp)
         r g fuel f_src f_tgt st_src st_tgt X itr_src ktr_tgt
     :
       bi_entails
-        (∀ x, back r g Q fuel f_src true (st_src, itr_src) (st_tgt, ktr_tgt x))
-        (back r g Q fuel f_src f_tgt (st_src, itr_src) (st_tgt, trigger (Choose X) >>= ktr_tgt)).
+        (∀ x, isim (r, g, f_src, true) Q fuel (st_src, itr_src) (st_tgt, ktr_tgt x))
+        (isim (r, g, f_src, f_tgt) Q fuel (st_src, itr_src) (st_tgt, trigger (Choose X) >>= ktr_tgt)).
   Proof.
-    eapply back_final. i. eapply hsimC_uclo. econs; eauto.
+    eapply isim_final. i. eapply hsimC_uclo. econs; eauto.
     inv CUR. red in IPROP. uipropall. i. eapply IPROP; eauto.
   Qed.
 
-  Lemma back_choose_tgt_trigger
+  Lemma isim_choose_tgt_trigger
         R_src X
         (Q: Any.t -> Any.t -> R_src -> X -> iProp)
         r g fuel f_src f_tgt st_src st_tgt itr_src
     :
       bi_entails
-        (∀ x, back r g Q fuel f_src true (st_src, itr_src) (st_tgt, Ret x))
-        (back r g Q fuel f_src f_tgt (st_src, itr_src) (st_tgt, trigger (Choose X))).
+        (∀ x, isim (r, g, f_src, true) Q fuel (st_src, itr_src) (st_tgt, Ret x))
+        (isim (r, g, f_src, f_tgt) Q fuel (st_src, itr_src) (st_tgt, trigger (Choose X))).
   Proof.
     erewrite (@idK_spec _ _ (trigger (Choose X))).
-    iIntros "H". iApply back_choose_tgt.
+    iIntros "H". iApply isim_choose_tgt.
     iIntros (x). iApply "H".
   Qed.
 
-  Lemma back_take_src
+  Lemma isim_take_src
         R_src R_tgt
         (Q: Any.t -> Any.t -> R_src -> R_tgt -> iProp)
         r g fuel f_src f_tgt st_src st_tgt X ktr_src itr_tgt
     :
       bi_entails
-        (∀ x, back r g Q None true f_tgt (st_src, ktr_src x) (st_tgt, itr_tgt))
-        (back r g Q fuel f_src f_tgt (st_src, trigger (Take X) >>= ktr_src) (st_tgt, itr_tgt)).
+        (∀ x, isim (r, g, true, f_tgt) Q None (st_src, ktr_src x) (st_tgt, itr_tgt))
+        (isim (r, g, f_src, f_tgt) Q fuel (st_src, trigger (Take X) >>= ktr_src) (st_tgt, itr_tgt)).
   Proof.
-    eapply back_final. i. eapply hsimC_uclo. econs; eauto.
+    eapply isim_final. i. eapply hsimC_uclo. econs; eauto.
     inv CUR. red in IPROP. uipropall. i. eapply IPROP; eauto.
   Qed.
 
-  Lemma back_take_src_trigger
+  Lemma isim_take_src_trigger
         X R_tgt
         (Q: Any.t -> Any.t -> X -> R_tgt -> iProp)
         r g fuel f_src f_tgt st_src st_tgt itr_tgt
     :
       bi_entails
-        (∀ x, back r g Q None true f_tgt (st_src, Ret x) (st_tgt, itr_tgt))
-        (back r g Q fuel f_src f_tgt (st_src, trigger (Take X)) (st_tgt, itr_tgt)).
+        (∀ x, isim (r, g, true, f_tgt) Q None (st_src, Ret x) (st_tgt, itr_tgt))
+        (isim (r, g, f_src, f_tgt) Q fuel (st_src, trigger (Take X)) (st_tgt, itr_tgt)).
   Proof.
     erewrite (@idK_spec _ _ (trigger (Take X))).
-    iIntros "H". iApply back_take_src.
+    iIntros "H". iApply isim_take_src.
     iIntros (x). iApply "H".
   Qed.
 
-  Lemma back_take_tgt
+  Lemma isim_take_tgt
         R_src R_tgt
         (Q: Any.t -> Any.t -> R_src -> R_tgt -> iProp)
         r g fuel f_src f_tgt st_src st_tgt X itr_src ktr_tgt
     :
       bi_entails
-        (∃ x, back r g Q fuel f_src true (st_src, itr_src) (st_tgt, ktr_tgt x))
-        (back r g Q fuel f_src f_tgt (st_src, itr_src) (st_tgt, trigger (Take X) >>= ktr_tgt)).
+        (∃ x, isim (r, g, f_src, true) Q fuel (st_src, itr_src) (st_tgt, ktr_tgt x))
+        (isim (r, g, f_src, f_tgt) Q fuel (st_src, itr_src) (st_tgt, trigger (Take X) >>= ktr_tgt)).
   Proof.
-    eapply back_final. i. eapply hsimC_uclo. econs; eauto.
+    eapply isim_final. i. eapply hsimC_uclo. econs; eauto.
     inv CUR. red in IPROP. uipropall. des. esplits. eapply IPROP; eauto.
   Qed.
 
-  Lemma back_take_tgt_trigger
+  Lemma isim_take_tgt_trigger
         R_src X
         (Q: Any.t -> Any.t -> R_src -> X -> iProp)
         r g fuel f_src f_tgt st_src st_tgt itr_src
     :
       bi_entails
-        (∃ x, back r g Q fuel f_src true (st_src, itr_src) (st_tgt, Ret x))
-        (back r g Q fuel f_src f_tgt (st_src, itr_src) (st_tgt, trigger (Take X))).
+        (∃ x, isim (r, g, f_src, true) Q fuel (st_src, itr_src) (st_tgt, Ret x))
+        (isim (r, g, f_src, f_tgt) Q fuel (st_src, itr_src) (st_tgt, trigger (Take X))).
   Proof.
     erewrite (@idK_spec _ _ (trigger (Take X))).
-    iIntros "H". iApply back_take_tgt.
+    iIntros "H". iApply isim_take_tgt.
     iDestruct "H" as (x) "H". iExists x. iApply "H".
   Qed.
 
-  Lemma back_pput_src
+  Lemma isim_pput_src
         R_src R_tgt
         (Q: Any.t -> Any.t -> R_src -> R_tgt -> iProp)
         r g fuel f_src f_tgt st_src0 st_src1 st_tgt ktr_src itr_tgt
     :
       bi_entails
-        (back r g Q None true f_tgt (st_src1, ktr_src tt) (st_tgt, itr_tgt))
-        (back r g Q fuel f_src f_tgt (st_src0, trigger (PPut st_src1) >>= ktr_src) (st_tgt, itr_tgt)).
+        (isim (r, g, true, f_tgt) Q None (st_src1, ktr_src tt) (st_tgt, itr_tgt))
+        (isim (r, g, f_src, f_tgt) Q fuel (st_src0, trigger (PPut st_src1) >>= ktr_src) (st_tgt, itr_tgt)).
   Proof.
-    eapply back_final. i. eapply hsimC_uclo. econs; eauto.
-    eapply back_current; eauto.
+    eapply isim_final. i. eapply hsimC_uclo. econs; eauto.
+    eapply isim_current; eauto.
   Qed.
 
-  Lemma back_pput_src_trigger
+  Lemma isim_pput_src_trigger
         R_tgt
         (Q: Any.t -> Any.t -> unit -> R_tgt -> iProp)
         r g fuel f_src f_tgt st_src0 st_src1 st_tgt itr_tgt
     :
       bi_entails
-        (back r g Q None true f_tgt (st_src1, Ret tt) (st_tgt, itr_tgt))
-        (back r g Q fuel f_src f_tgt (st_src0, trigger (PPut st_src1)) (st_tgt, itr_tgt)).
+        (isim (r, g, true, f_tgt) Q None (st_src1, Ret tt) (st_tgt, itr_tgt))
+        (isim (r, g, f_src, f_tgt) Q fuel (st_src0, trigger (PPut st_src1)) (st_tgt, itr_tgt)).
   Proof.
     erewrite (@idK_spec _ _ (trigger (PPut st_src1))).
-    iIntros "H". iApply back_pput_src. iApply "H".
+    iIntros "H". iApply isim_pput_src. iApply "H".
   Qed.
 
-  Lemma back_pget_src
+  Lemma isim_pget_src
         R_src R_tgt
         (Q: Any.t -> Any.t -> R_src -> R_tgt -> iProp)
         r g fuel f_src f_tgt st_src st_tgt ktr_src itr_tgt
     :
       bi_entails
-        (back r g Q None true f_tgt (st_src, ktr_src st_src) (st_tgt, itr_tgt))
-        (back r g Q fuel f_src f_tgt (st_src, trigger (PGet) >>= ktr_src) (st_tgt, itr_tgt)).
+        (isim (r, g, true, f_tgt) Q None (st_src, ktr_src st_src) (st_tgt, itr_tgt))
+        (isim (r, g, f_src, f_tgt) Q fuel (st_src, trigger (PGet) >>= ktr_src) (st_tgt, itr_tgt)).
   Proof.
-    eapply back_final. i. eapply hsimC_uclo. econs; eauto.
-    eapply back_current; eauto.
+    eapply isim_final. i. eapply hsimC_uclo. econs; eauto.
+    eapply isim_current; eauto.
   Qed.
 
-  Lemma back_get_src_trigger
+  Lemma isim_get_src_trigger
         R_tgt
         (Q: Any.t -> Any.t -> Any.t -> R_tgt -> iProp)
         r g fuel f_src f_tgt st_src st_tgt itr_tgt
     :
       bi_entails
-        (back r g Q None true f_tgt (st_src, Ret st_src) (st_tgt, itr_tgt))
-        (back r g Q fuel f_src f_tgt (st_src, trigger (PGet)) (st_tgt, itr_tgt)).
+        (isim (r, g, true, f_tgt) Q None (st_src, Ret st_src) (st_tgt, itr_tgt))
+        (isim (r, g, f_src, f_tgt) Q fuel (st_src, trigger (PGet)) (st_tgt, itr_tgt)).
   Proof.
     erewrite (@idK_spec _ _ (trigger (PGet))).
-    iIntros "H". iApply back_pget_src. iApply "H".
+    iIntros "H". iApply isim_pget_src. iApply "H".
   Qed.
 
-  Lemma back_pput_tgt
+  Lemma isim_pput_tgt
         R_src R_tgt
         (Q: Any.t -> Any.t -> R_src -> R_tgt -> iProp)
         r g fuel f_src f_tgt st_src st_tgt0 st_tgt1 itr_src ktr_tgt
     :
       bi_entails
-        (back r g Q fuel f_src true (st_src, itr_src) (st_tgt1, ktr_tgt tt))
-        (back r g Q fuel f_src f_tgt (st_src, itr_src) (st_tgt0, trigger (PPut st_tgt1) >>= ktr_tgt)).
+        (isim (r, g, f_src, true) Q fuel (st_src, itr_src) (st_tgt1, ktr_tgt tt))
+        (isim (r, g, f_src, f_tgt) Q fuel (st_src, itr_src) (st_tgt0, trigger (PPut st_tgt1) >>= ktr_tgt)).
   Proof.
-    eapply back_final. i. eapply hsimC_uclo. econs; eauto.
-    eapply back_current; eauto.
+    eapply isim_final. i. eapply hsimC_uclo. econs; eauto.
+    eapply isim_current; eauto.
   Qed.
 
-  Lemma back_pput_tgt_trigger
+  Lemma isim_pput_tgt_trigger
         R_src
         (Q: Any.t -> Any.t -> R_src -> unit -> iProp)
         r g fuel f_src f_tgt st_src st_tgt0 st_tgt1 itr_src
     :
       bi_entails
-        (back r g Q fuel f_src true (st_src, itr_src) (st_tgt1, Ret tt))
-        (back r g Q fuel f_src f_tgt (st_src, itr_src) (st_tgt0, trigger (PPut st_tgt1))).
+        (isim (r, g, f_src, true) Q fuel (st_src, itr_src) (st_tgt1, Ret tt))
+        (isim (r, g, f_src, f_tgt) Q fuel (st_src, itr_src) (st_tgt0, trigger (PPut st_tgt1))).
   Proof.
     erewrite (@idK_spec _ _ (trigger (PPut st_tgt1))).
-    iIntros "H". iApply back_pput_tgt. iApply "H".
+    iIntros "H". iApply isim_pput_tgt. iApply "H".
   Qed.
 
-  Lemma back_pget_tgt
+  Lemma isim_pget_tgt
         R_src R_tgt
         (Q: Any.t -> Any.t -> R_src -> R_tgt -> iProp)
         r g fuel f_src f_tgt st_src st_tgt itr_src ktr_tgt
     :
       bi_entails
-        (back r g Q fuel f_src true (st_src, itr_src) (st_tgt, ktr_tgt st_tgt))
-        (back r g Q fuel f_src f_tgt (st_src, itr_src) (st_tgt, trigger (PGet) >>= ktr_tgt)).
+        (isim (r, g, f_src, true) Q fuel (st_src, itr_src) (st_tgt, ktr_tgt st_tgt))
+        (isim (r, g, f_src, f_tgt) Q fuel (st_src, itr_src) (st_tgt, trigger (PGet) >>= ktr_tgt)).
   Proof.
-    eapply back_final. i. eapply hsimC_uclo. econs; eauto.
-    eapply back_current; eauto.
+    eapply isim_final. i. eapply hsimC_uclo. econs; eauto.
+    eapply isim_current; eauto.
   Qed.
 
-  Lemma back_pget_tgt_trigger
+  Lemma isim_pget_tgt_trigger
         R_src
         (Q: Any.t -> Any.t -> R_src -> Any.t -> iProp)
         r g fuel f_src f_tgt st_src st_tgt itr_src
     :
       bi_entails
-        (back r g Q fuel f_src true (st_src, itr_src) (st_tgt, Ret st_tgt))
-        (back r g Q fuel f_src f_tgt (st_src, itr_src) (st_tgt, trigger (PGet))).
+        (isim (r, g, f_src, true) Q fuel (st_src, itr_src) (st_tgt, Ret st_tgt))
+        (isim (r, g, f_src, f_tgt) Q fuel (st_src, itr_src) (st_tgt, trigger (PGet))).
   Proof.
     erewrite (@idK_spec _ _ (trigger (PGet))).
-    iIntros "H". iApply back_pget_tgt. iApply "H".
+    iIntros "H". iApply isim_pget_tgt. iApply "H".
   Qed.
 
-  Lemma back_assume_src
+  Lemma isim_assume_src
         R_src R_tgt
         (Q: Any.t -> Any.t -> R_src -> R_tgt -> iProp)
         r g fuel f_src f_tgt st_src st_tgt P k_src i_tgt
     :
       bi_entails
-        (⌜P⌝ -* back r g Q None true f_tgt (st_src, k_src tt) (st_tgt, i_tgt))
-        (back r g Q fuel f_src f_tgt (st_src, assume P >>= k_src) (st_tgt, i_tgt)).
+        (⌜P⌝ -* isim (r, g, true, f_tgt) Q None (st_src, k_src tt) (st_tgt, i_tgt))
+        (isim (r, g, f_src, f_tgt) Q fuel (st_src, assume P >>= k_src) (st_tgt, i_tgt)).
   Proof.
     iIntros "H". unfold assume. hred_l.
-    iApply back_take_src. iIntros (H). hred_l. iApply "H". iPureIntro. auto.
+    iApply isim_take_src. iIntros (H). hred_l. iApply "H". iPureIntro. auto.
   Qed.
 
-  Lemma back_assume_src_trigger
+  Lemma isim_assume_src_trigger
         R_tgt
         (Q: Any.t -> Any.t -> unit -> R_tgt -> iProp)
         r g fuel f_src f_tgt st_src st_tgt P itr_tgt
     :
       bi_entails
-        (⌜P⌝ -* back r g Q None true f_tgt (st_src, Ret tt) (st_tgt, itr_tgt))
-        (back r g Q fuel f_src f_tgt (st_src, assume P) (st_tgt, itr_tgt)).
+        (⌜P⌝ -* isim (r, g, true, f_tgt) Q None (st_src, Ret tt) (st_tgt, itr_tgt))
+        (isim (r, g, f_src, f_tgt) Q fuel (st_src, assume P) (st_tgt, itr_tgt)).
   Proof.
     erewrite (@idK_spec _ _ (assume P)).
-    iIntros "H". iApply back_assume_src.
+    iIntros "H". iApply isim_assume_src.
     iIntros "H0". iApply "H". auto.
   Qed.
 
-  Lemma back_assume_tgt
+  Lemma isim_assume_tgt
         R_src R_tgt
         (Q: Any.t -> Any.t -> R_src -> R_tgt -> iProp)
         r g fuel f_src f_tgt st_src st_tgt P itr_src ktr_tgt
     :
       bi_entails
-        (⌜P⌝ ∧ back r g Q fuel f_src true (st_src, itr_src) (st_tgt, ktr_tgt tt))
-        (back r g Q fuel f_src f_tgt (st_src, itr_src) (st_tgt, assume P >>= ktr_tgt)).
+        (⌜P⌝ ∧ isim (r, g, f_src, true) Q fuel (st_src, itr_src) (st_tgt, ktr_tgt tt))
+        (isim (r, g, f_src, f_tgt) Q fuel (st_src, itr_src) (st_tgt, assume P >>= ktr_tgt)).
   Proof.
     iIntros "H". iDestruct "H" as "[% H]".
-    unfold assume. hred_r. iApply back_take_tgt.
+    unfold assume. hred_r. iApply isim_take_tgt.
     iExists H. hred_r. iApply "H".
   Qed.
 
@@ -841,241 +837,241 @@ Section SIM.
     iApply "H1". iApply "H0".
   Qed.
 
-  Lemma back_assume_tgt_trigger
+  Lemma isim_assume_tgt_trigger
         R_src
         (Q: Any.t -> Any.t -> R_src -> unit -> iProp)
         r g fuel f_src f_tgt st_src st_tgt P itr_src
     :
       bi_entails
-        (⌜P⌝ ∧ back r g Q fuel f_src true (st_src, itr_src) (st_tgt, Ret tt))
-        (back r g Q fuel f_src f_tgt (st_src, itr_src) (st_tgt, assume P)).
+        (⌜P⌝ ∧ isim (r, g, f_src, true) Q fuel (st_src, itr_src) (st_tgt, Ret tt))
+        (isim (r, g, f_src, f_tgt) Q fuel (st_src, itr_src) (st_tgt, assume P)).
   Proof.
     erewrite (@idK_spec _ _ (assume P)).
-    iIntros "H". iApply back_assume_tgt. iSplit; auto.
+    iIntros "H". iApply isim_assume_tgt. iSplit; auto.
     { iDestruct "H" as "[H _]". iApply "H". }
     { iDestruct "H" as "[_ H]". iApply "H". }
   Qed.
 
-  Lemma back_guarantee_src
+  Lemma isim_guarantee_src
         R_src R_tgt
         (Q: Any.t -> Any.t -> R_src -> R_tgt -> iProp)
         r g fuel f_src f_tgt st_src st_tgt P ktr_src itr_tgt
     :
       bi_entails
-        (⌜P⌝ ∧ back r g Q None true f_tgt (st_src, ktr_src tt) (st_tgt, itr_tgt))
-        (back r g Q fuel f_src f_tgt (st_src, guarantee P >>= ktr_src) (st_tgt, itr_tgt)).
+        (⌜P⌝ ∧ isim (r, g, true, f_tgt) Q None (st_src, ktr_src tt) (st_tgt, itr_tgt))
+        (isim (r, g, f_src, f_tgt) Q fuel (st_src, guarantee P >>= ktr_src) (st_tgt, itr_tgt)).
   Proof.
     iIntros "H". iDestruct "H" as "[% H]".
-    unfold guarantee. hred_l. iApply back_choose_src.
+    unfold guarantee. hred_l. iApply isim_choose_src.
     iExists H. hred_l. iApply "H".
   Qed.
 
-  Lemma back_guarantee_src_trigger
+  Lemma isim_guarantee_src_trigger
         R_tgt
         (Q: Any.t -> Any.t -> unit -> R_tgt -> iProp)
         r g fuel f_src f_tgt st_src st_tgt P itr_tgt
     :
       bi_entails
-        (⌜P⌝ ∧ back r g Q None true f_tgt (st_src, Ret tt) (st_tgt, itr_tgt))
-        (back r g Q fuel f_src f_tgt (st_src, guarantee P) (st_tgt, itr_tgt)).
+        (⌜P⌝ ∧ isim (r, g, true, f_tgt) Q None (st_src, Ret tt) (st_tgt, itr_tgt))
+        (isim (r, g, f_src, f_tgt) Q fuel (st_src, guarantee P) (st_tgt, itr_tgt)).
   Proof.
     erewrite (@idK_spec _ _ (guarantee P)).
-    iIntros "H". iApply back_guarantee_src. iSplit; auto.
+    iIntros "H". iApply isim_guarantee_src. iSplit; auto.
     { iDestruct "H" as "[H _]". iApply "H". }
     { iDestruct "H" as "[_ H]". iApply "H". }
   Qed.
 
-  Lemma back_guarantee_tgt
+  Lemma isim_guarantee_tgt
         R_src R_tgt
         (Q: Any.t -> Any.t -> R_src -> R_tgt -> iProp)
         r g fuel f_src f_tgt st_src st_tgt P itr_src ktr_tgt
     :
       bi_entails
-        (⌜P⌝ -* back r g Q fuel f_src true (st_src, itr_src) (st_tgt, ktr_tgt tt))
-        (back r g Q fuel f_src f_tgt (st_src, itr_src) (st_tgt, guarantee P >>= ktr_tgt)).
+        (⌜P⌝ -* isim (r, g, f_src, true) Q fuel (st_src, itr_src) (st_tgt, ktr_tgt tt))
+        (isim (r, g, f_src, f_tgt) Q fuel (st_src, itr_src) (st_tgt, guarantee P >>= ktr_tgt)).
   Proof.
     iIntros "H". unfold guarantee. hred_r.
-    iApply back_choose_tgt.
+    iApply isim_choose_tgt.
     iIntros (H). hred_r. iApply "H". iPureIntro. auto.
   Qed.
 
-  Lemma back_guarantee_tgt_trigger
+  Lemma isim_guarantee_tgt_trigger
         R_src
         (Q: Any.t -> Any.t -> R_src -> unit -> iProp)
         r g fuel f_src f_tgt st_src st_tgt P itr_src
     :
       bi_entails
-        (⌜P⌝ -* back r g Q fuel f_src true (st_src, itr_src) (st_tgt, Ret tt))
-        (back r g Q fuel f_src f_tgt (st_src, itr_src) (st_tgt, guarantee P)).
+        (⌜P⌝ -* isim (r, g, f_src, true) Q fuel (st_src, itr_src) (st_tgt, Ret tt))
+        (isim (r, g, f_src, f_tgt) Q fuel (st_src, itr_src) (st_tgt, guarantee P)).
   Proof.
     erewrite (@idK_spec _ _ (guarantee P)).
-    iIntros "H". iApply back_guarantee_tgt.
+    iIntros "H". iApply isim_guarantee_tgt.
     iIntros "H0". iApply "H". auto.
   Qed.
 
-  Lemma back_triggerUB_src
+  Lemma isim_triggerUB_src
         R_src R_tgt
         (Q: Any.t -> Any.t -> R_src -> R_tgt -> iProp)
         r g fuel f_src f_tgt st_src st_tgt X (ktr_src: X -> _) itr_tgt
     :
       bi_entails
         (⌜True⌝)
-        (back r g Q fuel f_src f_tgt (st_src, triggerUB >>= ktr_src) (st_tgt, itr_tgt)).
+        (isim (r, g, f_src, f_tgt) Q fuel (st_src, triggerUB >>= ktr_src) (st_tgt, itr_tgt)).
   Proof.
-    iIntros "H". unfold triggerUB. hred_l. iApply back_take_src.
+    iIntros "H". unfold triggerUB. hred_l. iApply isim_take_src.
     iIntros (x). destruct x.
   Qed.
 
-  Lemma back_triggerUB_src_trigger
+  Lemma isim_triggerUB_src_trigger
         R_src R_tgt
         (Q: Any.t -> Any.t -> R_src -> R_tgt -> iProp)
         r g fuel f_src f_tgt st_src st_tgt itr_tgt
     :
       bi_entails
         (⌜True⌝)
-        (back r g Q fuel f_src f_tgt (st_src, triggerUB) (st_tgt, itr_tgt)).
+        (isim (r, g, f_src, f_tgt) Q fuel (st_src, triggerUB) (st_tgt, itr_tgt)).
   Proof.
     erewrite (@idK_spec _ _ (triggerUB)).
-    iIntros "H". iApply back_triggerUB_src. auto.
+    iIntros "H". iApply isim_triggerUB_src. auto.
   Qed.
 
-  Lemma back_triggerNB_tgt
+  Lemma isim_triggerNB_tgt
         R_src R_tgt
         (Q: Any.t -> Any.t -> R_src -> R_tgt -> iProp)
         r g fuel f_src f_tgt st_src st_tgt X itr_src (ktr_tgt: X -> _)
     :
       bi_entails
         (⌜True⌝)
-        (back r g Q fuel f_src f_tgt (st_src, itr_src) (st_tgt, triggerNB >>= ktr_tgt)).
+        (isim (r, g, f_src, f_tgt) Q fuel (st_src, itr_src) (st_tgt, triggerNB >>= ktr_tgt)).
   Proof.
-    iIntros "H". unfold triggerNB. hred_r. iApply back_choose_tgt.
+    iIntros "H". unfold triggerNB. hred_r. iApply isim_choose_tgt.
     iIntros (x). destruct x.
   Qed.
 
-  Lemma back_triggerNB_trigger
+  Lemma isim_triggerNB_trigger
         R_src R_tgt
         (Q: Any.t -> Any.t -> R_src -> R_tgt -> iProp)
         r g fuel f_src f_tgt st_src st_tgt itr_src
     :
       bi_entails
         (⌜True⌝)
-        (back r g Q fuel f_src f_tgt (st_src, itr_src) (st_tgt, triggerNB)).
+        (isim (r, g, f_src, f_tgt) Q fuel (st_src, itr_src) (st_tgt, triggerNB)).
   Proof.
     erewrite (@idK_spec _ _ (triggerNB)).
-    iIntros "H". iApply back_triggerNB_tgt. auto.
+    iIntros "H". iApply isim_triggerNB_tgt. auto.
   Qed.
 
-  Lemma back_unwrapU_src
+  Lemma isim_unwrapU_src
         R_src R_tgt
         (Q: Any.t -> Any.t -> R_src -> R_tgt -> iProp)
         r g fuel f_src f_tgt st_src st_tgt X (x: option X) ktr_src itr_tgt
     :
       bi_entails
-        (∀ x', ⌜x = Some x'⌝ -* back r g Q fuel f_src f_tgt (st_src, ktr_src x') (st_tgt, itr_tgt))
-        (back r g Q fuel f_src f_tgt (st_src, unwrapU x >>= ktr_src) (st_tgt, itr_tgt)).
+        (∀ x', ⌜x = Some x'⌝ -* isim (r, g, f_src, f_tgt) Q fuel (st_src, ktr_src x') (st_tgt, itr_tgt))
+        (isim (r, g, f_src, f_tgt) Q fuel (st_src, unwrapU x >>= ktr_src) (st_tgt, itr_tgt)).
   Proof.
     iIntros "H". unfold unwrapU. destruct x.
     { hred_l. iApply "H". auto. }
-    { iApply back_triggerUB_src. auto. }
+    { iApply isim_triggerUB_src. auto. }
   Qed.
 
-  Lemma back_unwrapU_src_trigger
+  Lemma isim_unwrapU_src_trigger
         X R_tgt
         (Q: Any.t -> Any.t -> X -> R_tgt -> iProp)
         r g fuel f_src f_tgt st_src st_tgt x itr_tgt
     :
       bi_entails
-        (∀ x', ⌜x = Some x'⌝ -* back r g Q fuel f_src f_tgt (st_src, Ret x') (st_tgt, itr_tgt))
-        (back r g Q fuel f_src f_tgt (st_src, unwrapU x) (st_tgt, itr_tgt)).
+        (∀ x', ⌜x = Some x'⌝ -* isim (r, g, f_src, f_tgt) Q fuel (st_src, Ret x') (st_tgt, itr_tgt))
+        (isim (r, g, f_src, f_tgt) Q fuel (st_src, unwrapU x) (st_tgt, itr_tgt)).
   Proof.
     erewrite (@idK_spec _ _ (unwrapU x)).
-    iIntros "H". iApply back_unwrapU_src.
+    iIntros "H". iApply isim_unwrapU_src.
     iIntros (x') "EQ". iApply "H"; auto.
   Qed.
 
-  Lemma back_unwrapN_src
+  Lemma isim_unwrapN_src
         R_src R_tgt
         (Q: Any.t -> Any.t -> R_src -> R_tgt -> iProp)
         r g fuel f_src f_tgt st_src st_tgt X (x: option X) ktr_src itr_tgt
     :
       bi_entails
-        (∃ x', ⌜x = Some x'⌝ ∧ back r g Q fuel f_src f_tgt (st_src, ktr_src x') (st_tgt, itr_tgt))
-        (back r g Q fuel f_src f_tgt (st_src, unwrapN x >>= ktr_src) (st_tgt, itr_tgt)).
+        (∃ x', ⌜x = Some x'⌝ ∧ isim (r, g, f_src, f_tgt) Q fuel (st_src, ktr_src x') (st_tgt, itr_tgt))
+        (isim (r, g, f_src, f_tgt) Q fuel (st_src, unwrapN x >>= ktr_src) (st_tgt, itr_tgt)).
   Proof.
     iIntros "H". iDestruct "H" as (x') "[% H]".
-    subst. ss. hred_l. iApply "H".
+    subst. hred_l. iApply "H".
   Qed.
 
-  Lemma back_unwrapN_src_trigger
+  Lemma isim_unwrapN_src_trigger
         R_src R_tgt
         (Q: Any.t -> Any.t -> R_src -> R_tgt -> iProp)
         r g fuel f_src f_tgt st_src st_tgt x itr_tgt
     :
       bi_entails
-        (∃ x', ⌜x = Some x'⌝ ∧ back r g Q fuel f_src f_tgt (st_src, Ret x') (st_tgt, itr_tgt))
-        (back r g Q fuel f_src f_tgt (st_src, unwrapN x) (st_tgt, itr_tgt)).
+        (∃ x', ⌜x = Some x'⌝ ∧ isim (r, g, f_src, f_tgt) Q fuel (st_src, Ret x') (st_tgt, itr_tgt))
+        (isim (r, g, f_src, f_tgt) Q fuel (st_src, unwrapN x) (st_tgt, itr_tgt)).
   Proof.
     erewrite (@idK_spec _ _ (unwrapN x)).
     iIntros "H". iDestruct "H" as (x') "[% H]".
-    iApply back_unwrapN_src. iExists x'. iSplit; auto.
+    iApply isim_unwrapN_src. iExists x'. iSplit; auto.
   Qed.
 
-  Lemma back_unwrapU_tgt
+  Lemma isim_unwrapU_tgt
         R_src R_tgt
         (Q: Any.t -> Any.t -> R_src -> R_tgt -> iProp)
         r g fuel f_src f_tgt st_src st_tgt X (x: option X) itr_src ktr_tgt
     :
       bi_entails
-        (∃ x', ⌜x = Some x'⌝ ∧ back r g Q fuel f_src f_tgt (st_src, itr_src) (st_tgt, ktr_tgt x'))
-        (back r g Q fuel f_src f_tgt (st_src, itr_src) (st_tgt, unwrapU x >>= ktr_tgt)).
+        (∃ x', ⌜x = Some x'⌝ ∧ isim (r, g, f_src, f_tgt) Q fuel (st_src, itr_src) (st_tgt, ktr_tgt x'))
+        (isim (r, g, f_src, f_tgt) Q fuel (st_src, itr_src) (st_tgt, unwrapU x >>= ktr_tgt)).
   Proof.
-    iIntros "H". iDestruct "H" as (x') "[% H]". subst. ss.
+    iIntros "H". iDestruct "H" as (x') "[% H]". subst.
     hred_r. iApply "H".
   Qed.
 
-  Lemma back_unwrapU_tgt_trigger
+  Lemma isim_unwrapU_tgt_trigger
         R_src R_tgt
         (Q: Any.t -> Any.t -> R_src -> R_tgt -> iProp)
         r g fuel f_src f_tgt st_src st_tgt x itr_src
     :
       bi_entails
-        (∃ x', ⌜x = Some x'⌝ ∧ back r g Q fuel f_src f_tgt (st_src, itr_src) (st_tgt, Ret x'))
-        (back r g Q fuel f_src f_tgt (st_src, itr_src) (st_tgt, unwrapU x)).
+        (∃ x', ⌜x = Some x'⌝ ∧ isim (r, g, f_src, f_tgt) Q fuel (st_src, itr_src) (st_tgt, Ret x'))
+        (isim (r, g, f_src, f_tgt) Q fuel (st_src, itr_src) (st_tgt, unwrapU x)).
   Proof.
     erewrite (@idK_spec _ _ (unwrapU x)).
     iIntros "H". iDestruct "H" as (x') "[% H]".
-    iApply back_unwrapU_tgt. iExists x'. iSplit; auto.
+    iApply isim_unwrapU_tgt. iExists x'. iSplit; auto.
   Qed.
 
-  Lemma back_unwrapN_tgt
+  Lemma isim_unwrapN_tgt
         R_src R_tgt
         (Q: Any.t -> Any.t -> R_src -> R_tgt -> iProp)
         r g fuel f_src f_tgt st_src st_tgt X (x: option X) itr_src ktr_tgt
     :
       bi_entails
-        (∀ x', ⌜x = Some x'⌝ -* back r g Q fuel f_src f_tgt (st_src, itr_src) (st_tgt, ktr_tgt x'))
-        (back r g Q fuel f_src f_tgt (st_src, itr_src) (st_tgt, unwrapN x >>= ktr_tgt)).
+        (∀ x', ⌜x = Some x'⌝ -* isim (r, g, f_src, f_tgt) Q fuel (st_src, itr_src) (st_tgt, ktr_tgt x'))
+        (isim (r, g, f_src, f_tgt) Q fuel (st_src, itr_src) (st_tgt, unwrapN x >>= ktr_tgt)).
   Proof.
     iIntros "H". unfold unwrapN. destruct x.
     { hred_r. iApply "H". auto. }
-    { iApply back_triggerNB_tgt. auto. }
+    { iApply isim_triggerNB_tgt. auto. }
   Qed.
 
-  Lemma back_unwrapN_tgt_trigger
+  Lemma isim_unwrapN_tgt_trigger
         R_src R_tgt
         (Q: Any.t -> Any.t -> R_src -> R_tgt -> iProp)
         r g fuel f_src f_tgt st_src st_tgt x itr_src
     :
       bi_entails
-        (∀ x', ⌜x = Some x'⌝ -* back r g Q fuel f_src f_tgt (st_src, itr_src) (st_tgt, Ret x'))
-        (back r g Q fuel f_src f_tgt (st_src, itr_src) (st_tgt, unwrapN x)).
+        (∀ x', ⌜x = Some x'⌝ -* isim (r, g, f_src, f_tgt) Q fuel (st_src, itr_src) (st_tgt, Ret x'))
+        (isim (r, g, f_src, f_tgt) Q fuel (st_src, itr_src) (st_tgt, unwrapN x)).
   Proof.
     erewrite (@idK_spec _ _ (unwrapN x)).
-    iIntros "H". iApply back_unwrapN_tgt.
+    iIntros "H". iApply isim_unwrapN_tgt.
     iIntros (x') "EQ". iApply "H"; auto.
   Qed.
 
-  Lemma back_ccallU_pure
+  Lemma isim_ccallU_pure
         pre post w0 fuel1
         R_src R_tgt
         (Q: Any.t -> Any.t -> R_src -> R_tgt -> iProp)
@@ -1090,10 +1086,10 @@ Section SIM.
                   ** (pre: iProp)
                   **
                   (∀ st_src st_tgt ret_src ret_tgt,
-                      ((inv_with le I w0 st_src st_tgt) ** (post ret_src ret_tgt: iProp)) -* ∃ ret_tgt', ⌜ret_tgt = Any.upcast ret_tgt'⌝ ∧ back g g Q (Some fuel1) true true (st_src, itr_src) (st_tgt, ktr_tgt ret_tgt')))
-        (back r g Q (Some fuel0) f_src f_tgt (st_src, itr_src) (st_tgt, ccallU fn arg_tgt >>= ktr_tgt)).
+                      ((inv_with le I w0 st_src st_tgt) ** (post ret_src ret_tgt: iProp)) -* ∃ ret_tgt', ⌜ret_tgt = Any.upcast ret_tgt'⌝ ∧ isim (g, g, true, true) Q (Some fuel1) (st_src, itr_src) (st_tgt, ktr_tgt ret_tgt')))
+        (isim (r, g, f_src, f_tgt) Q (Some fuel0) (st_src, itr_src) (st_tgt, ccallU fn arg_tgt >>= ktr_tgt)).
   Proof.
-    iIntros "[H0 H1]". unfold ccallU. hred_r. iApply back_call_pure; eauto.
+    iIntros "[H0 H1]". unfold ccallU. hred_r. iApply isim_call_pure; eauto.
     iSplitL "H0"; [iExact "H0"|].
     iIntros (st_src0 st_tgt0 ret_src ret_tgt) "H0".
     iPoseProof ("H1" with "H0") as (ret_tgt') "[% H1]". subst.
@@ -1101,25 +1097,28 @@ Section SIM.
   Qed.
 End SIM.
 
+Global Opaque isim.
+
 Require Import OpenDef.
 
 Section ADEQUACY.
   Context `{Σ: GRA.t}.
 
-  Lemma back_fun_to_tgt_aux
+  Lemma isim_fun_to_tgt_aux
         A wf (le: A -> A -> Prop) `{PreOrder _ le} mn stb
         f_src f_tgt w
         (fsp: fspecbody) x y f st_src st_tgt
         (EQ: x = y)
         (WF: mk_wf wf w (st_src, st_tgt))
-        (BACK: forall w (x: fsp.(meta)) mn_caller arg_src arg_tgt st_src st_tgt,
+        (ISIM: forall w (x: fsp.(meta)) mn_caller arg_src arg_tgt st_src st_tgt,
             bi_entails
               ((inv_with le wf w st_src st_tgt) ** (fsp.(precond) mn_caller x arg_src arg_tgt: iProp))
-              (back
-                 le wf mn stb (fsp.(measure) x) bot9 bot9
+              (isim
+                 le wf mn stb (fsp.(measure) x)
+                 (bot9, bot9, true, f_tgt)
                  (fun st_src st_tgt ret_src ret_tgt =>
                     (inv_with le wf w st_src st_tgt) ** (fsp.(postcond) mn_caller x ret_src ret_tgt: iProp))
-                 None true f_tgt
+                 None
                  (st_src, match fsp.(measure) x with
                           | ord_pure _ => _ <- trigger hAPC;; trigger (Choose Any.t)
                           | ord_top => fsp.(fsb_body) (mn_caller, arg_src)
@@ -1134,22 +1133,23 @@ Section ADEQUACY.
     subst. destruct y as [mn_caller arg].
     ginit. unfold fun_to_tgt. rewrite HoareFun_parse. harg.
     gfinal. right. eapply hsim_adequacy; auto.
-    ginit. eapply back_init; [clear ACC|eapply ACC]. start_ipm_proof.
-    iApply BACK. iSplitR "PRE"; [|iExact "PRE"].
+    ginit. eapply isim_init; [clear ACC|eapply ACC]. start_ipm_proof.
+    iApply ISIM. iSplitR "PRE"; [|iExact "PRE"].
     iExists w. iSplit; auto.
   Qed.
 
-  Lemma back_fun_to_tgt
+  Lemma isim_fun_to_tgt
         A wf (le: A -> A -> Prop) `{PreOrder _ le} mn stb
         (fsp: fspecbody) f
-        (BACK: forall w (x: fsp.(meta)) mn_caller arg_src arg_tgt st_src st_tgt,
+        (ISIM: forall w (x: fsp.(meta)) mn_caller arg_src arg_tgt st_src st_tgt,
             bi_entails
               ((inv_with le wf w st_src st_tgt) ** (fsp.(precond) mn_caller x arg_src arg_tgt: iProp))
-              (back
-                 le wf mn stb (fsp.(measure) x) bot9 bot9
+              (isim
+                 le wf mn stb (fsp.(measure) x)
+                 (bot9, bot9, true, false)
                  (fun st_src st_tgt ret_src ret_tgt =>
                     (inv_with le wf w st_src st_tgt) ** (fsp.(postcond) mn_caller x ret_src ret_tgt: iProp))
-                 None true false
+                 None
                  (st_src, match fsp.(measure) x with
                           | ord_pure _ => _ <- trigger hAPC;; trigger (Choose Any.t)
                           | ord_top => fsp.(fsb_body) (mn_caller, arg_src)
@@ -1158,20 +1158,21 @@ Section ADEQUACY.
       sim_fsem (mk_wf wf) le
                (fun_to_tgt mn stb fsp) f.
   Proof.
-    ii. eapply back_fun_to_tgt_aux; eauto.
+    ii. eapply isim_fun_to_tgt_aux; eauto.
   Qed.
 
-  Lemma back_fun_to_tgt_open
+  Lemma isim_fun_to_tgt_open
         A wf (le: A -> A -> Prop) `{PreOrder _ le} mn stb
         (ksp: kspecbody) f
         (FRIEND: forall w (x: ksp.(meta)) mn_caller arg_src arg_tgt st_src st_tgt,
             bi_entails
               ((inv_with le wf w st_src st_tgt) ** (ksp.(precond) mn_caller x arg_src arg_tgt: iProp))
-              (back
-                 le wf mn stb (ksp.(measure) x) bot9 bot9
+              (isim
+                 le wf mn stb (ksp.(measure) x)
+                 (bot9, bot9, true, false)
                  (fun st_src st_tgt ret_src ret_tgt =>
                     (inv_with le wf w st_src st_tgt) ** (ksp.(postcond) mn_caller x ret_src ret_tgt: iProp))
-                 None true false
+                 None
                  (st_src, match ksp.(measure) x with
                           | ord_pure _ => _ <- trigger hAPC;; trigger (Choose Any.t)
                           | ord_top => ksp.(ksb_kbody) (mn_caller, arg_src)
@@ -1179,11 +1180,12 @@ Section ADEQUACY.
         (CONTEXT: forall w mn_caller arg st_src st_tgt,
             bi_entails
               (inv_with le wf w st_src st_tgt)
-              (back
-                 le wf mn stb ord_top bot9 bot9
+              (isim
+                 le wf mn stb ord_top
+                 (bot9, bot9, true, false)
                  (fun st_src st_tgt ret_src ret_tgt =>
                     (inv_with le wf w st_src st_tgt ** ⌜ret_src = ret_tgt⌝))
-                 None true false
+                 None
                  (st_src, ksp.(ksb_ubody) (mn_caller, arg)) (st_tgt, f (mn_caller, arg))))
     :
       sim_fsem (mk_wf wf) le
@@ -1191,29 +1193,30 @@ Section ADEQUACY.
   Proof.
     ii. ginit. unfold KModSem.disclose_ksb_tgt.
     apply sim_itreeC_spec. apply sim_itreeC_take_src. intros [].
-    { gfinal. right. eapply back_fun_to_tgt_aux; eauto. }
-    { gfinal. right. eapply back_fun_to_tgt_aux; eauto. i. ss.
+    { gfinal. right. eapply isim_fun_to_tgt_aux; eauto. }
+    { gfinal. right. eapply isim_fun_to_tgt_aux; eauto. i. ss.
       iIntros "[H0 %]". subst. iApply CONTEXT. auto.
     }
   Qed.
 
-  Lemma back_fun_to_tgt_open_trivial
+  Lemma isim_fun_to_tgt_open_trivial
         A wf (le: A -> A -> Prop) `{PreOrder _ le} mn stb
         body f
         (CONTEXT: forall w mn_caller arg st_src st_tgt,
             bi_entails
               (inv_with le wf w st_src st_tgt)
-              (back
-                 le wf mn stb ord_top bot9 bot9
+              (isim
+                 le wf mn stb ord_top
+                 (bot9, bot9, true, false)
                  (fun st_src st_tgt ret_src ret_tgt =>
                     (inv_with le wf w st_src st_tgt ** ⌜ret_src = ret_tgt⌝))
-                 None true false
+                 None
                  (st_src, body (mn_caller, arg)) (st_tgt, f (mn_caller, arg))))
     :
       sim_fsem (mk_wf wf) le
                (KModSem.disclose_ksb_tgt mn stb (ksb_trivial body)) f.
   Proof.
-    eapply back_fun_to_tgt_open; ss; auto. i.
+    eapply isim_fun_to_tgt_open; ss; auto. i.
     iIntros "[H0 %]". subst. iApply CONTEXT. iApply "H0".
   Qed.
 End ADEQUACY.
