examples/cannon/Cannon01proofH.v
@@ -1,0 +1,63 @@
+Require Import HoareDef STB CannonRA Cannon0 Cannon1 SimModSem.
+Require Import Coqlib.
+Require Import ImpPrelude.
+Require Import Skeleton.
+Require Import PCM.
+Require Import ModSem Behavior.
+Require Import HTactics ProofMode.
+Require Import HSim IProofMode.
+
+Set Implicit Arguments.
+
+
+
+Section SIMMODSEM.
+
+  Context `{Σ: GRA.t}.
+  Context `{@GRA.inG CannonRA Σ}.
+
+  Let W: Type := Any.t * Any.t.
+
+  Variable GlobalStb: Sk.t -> gname -> option fspec.
+
+  Let wf: unit -> Any.t -> Any.t -> iProp :=
+    (fun (_: unit) st_src st_tgt => ((⌜st_src = (1: Z)↑ /\ st_tgt = (1: Z)↑⌝ ** OwnM (Ready))
+                                     ∨ OwnM (Fired))%I)
+  .
+
+  Let top2_PreOrder: @PreOrder unit top2.
+  Proof. econs; eauto. Qed.
+  Local Existing Instance top2_PreOrder.
+
+  Theorem correct: refines2 [Cannon0.Cannon] [Cannon1.Cannon GlobalStb].
+  Proof.
+    eapply adequacy_local2. econs; ss.
+    i. econstructor 1 with (le:=top2) (wf:=mk_wf wf); et; ss; cycle 1.
+    { exists tt. econs. eapply to_semantic.
+      iIntros "H". iLeft. iSplitR; ss. }
+    econs; ss. econs; ss.
+    apply isim_fun_to_tgt; auto. i; ss.
+    unfold Cannon0.fire_body, Cannon1.fire_body.
+    iIntros "[INV PRE]".
+    iDestruct "PRE" as "[[% BALL] %]". subst.
+    iEval (unfold inv_with, wf) in "INV".
+    iDestruct "INV" as (w1) "[[[% READY] | FIRED] _]".
+    { des; subst. hred_l. hred_r.
+      iApply isim_pget_tgt. hred_r.
+      iApply isim_syscall. iIntros (_).
+      hred_l. hred_r.
+      iApply isim_pput_tgt. hred_r.
+      iApply isim_ret. iSplit.
+      { iApply inv_with_current. iEval (unfold wf).
+        iRight. iCombine "READY" "BALL" as "FIRED".
+        iEval (rewrite <- ReadyBall). iApply "FIRED".
+      }
+      { iPureIntro. auto. }
+    }
+    { iCombine "FIRED" "BALL" as "FALSE".
+      iPoseProof (OwnM_valid with "FALSE") as "%".
+      exfalso. eapply FiredBall; auto.
+    }
+  Qed.
+
+End SIMMODSEM.
